NuSys.thy
@@ -5,9 +5,10 @@ theory NuSys
   keywords
     "proc" :: thy_decl_block
   and "\<medium_left_bracket>" "as" "\<rightarrow>" "\<longmapsto>" :: quasi_command
-  and "\<bullet>" "--" :: prf_decl % "proof"
+  and "\<bullet>" "premise" :: prf_decl % "proof"
   and "\<nu>processor" "\<nu>processor_resolver" :: thy_decl % "ML"
   and "\<nu>procedure" :: thy_decl
+  and "finish" :: qed_block % "proof"
 abbrevs
   "!!" = "!!"
 begin
@@ -38,22 +39,26 @@ attribute_setup show_proc_expression = \<open>NuToplevel.show_proc_expression_at
 
 ML \<open>
 
-local open Parse Scan NuToplevel NuSys in
+local open Scan NuToplevel NuSys Parse in
 val bracket_begin = $$$ "\<medium_left_bracket>";
 
 val _ =
   Outer_Syntax.local_theory_to_proof' \<^command_keyword>\<open>proc\<close> "begin a procedure construction"
     ((Parse_Spec.thm_name ":" -- Parse.term --| $$$ "\<longmapsto>" -- Parse.term -- Parse.for_fixes -- Scan.optional Parse_Spec.includes []
-            -- Parse_Spec.if_statement) --| bracket_begin >>
+            -- Parse_Spec.if_statement) --| $$$ "begin" >>
         (fn (((((b,arg),ret),fixes),includes),preconds) =>  
             (begin_proc_cmd b arg ret fixes includes preconds)));
+
+val _ =
+  Outer_Syntax.command \<^command_keyword>\<open>finish\<close> "Finish the procedure construction"
+    (Scan.succeed NuToplevel.finish_proc_cmd)
 
 val _ =
   Outer_Syntax.command \<^command_keyword>\<open>\<bullet>\<close> "The \<nu>construction"
     (fn toks => (Toplevel.proof (NuToplevel.process_cmd (toks @ [Token.eof])), []))
 
 val _ =
-  Outer_Syntax.command \<^command_keyword>\<open>--\<close> "assign registers"
+  Outer_Syntax.command \<^command_keyword>\<open>premise\<close> "proof for premise"
     (Scan.succeed (Toplevel.proof NuToplevel.prove_prem))
 
 val _ =
@@ -68,7 +73,7 @@ val _ =
 
 val _ =
   Outer_Syntax.local_theory \<^command_keyword>\<open>\<nu>procedure\<close> "declare \<nu>procedure"
-    (Parse.binding >> (Context.proof_map o NuProcedure.declare))
+    (and_list1 binding >> (Context.proof_map o fold NuProcedure.declare))
 
 end
 \<close>
@@ -78,19 +83,26 @@ attribute_setup \<nu>proc = \<open>Scan.lift (Parse.name_position) >> (fn name =
   then (NONE, SOME (foldr1 (uncurry Conjunction.intr) (NuProcedure.check ctx name)))
   else (SOME (NuProcedure.define name th ctx), NONE))\<close>
 
-\<nu>processor set_auto_level 10 \<open>PROP P\<close> \<open>(fn auto_level => fn ctx => fn th => NuParse.auto_level_force #->
-  (fn auto_level' => NuProcessor.process (Int.min (auto_level, auto_level')) ctx th #> (fn x => raise ProcessTerminated x)))\<close>
+(* \<nu>processor set_auto_level 10 \<open>PROP P\<close> \<open>(fn auto_level => fn ctx => fn th => NuParse.auto_level_force #->
+  (fn auto_level' => NuProcessor.process (Int.min (auto_level, auto_level')) ctx th #> (fn x => raise ProcessTerminated x)))\<close> *)
 \<nu>processor accept_proc 300 \<open>\<^bold>p\<^bold>e\<^bold>n\<^bold>d\<^bold>i\<^bold>n\<^bold>g f \<^bold>o\<^bold>n blk \<^bold>r\<^bold>e\<^bold>s\<^bold>u\<^bold>l\<^bold>t\<^bold>s \<^bold>i\<^bold>n T\<close> \<open>safe (Scan.succeed oo NuSys.accept_proc)\<close>
 \<nu>processor assign_register 500 \<open>\<^bold>c\<^bold>u\<^bold>r\<^bold>r\<^bold>e\<^bold>n\<^bold>t blk \<^bold>r\<^bold>e\<^bold>s\<^bold>u\<^bold>l\<^bold>t\<^bold>s \<^bold>i\<^bold>n T\<close>  \<open>let open Parse in
   (fn auto_level => fn ctx => fn th => ($$$ "\<rightarrow>" |-- (short_ident >> single || $$$ "(" |-- list1 short_ident --| $$$ ")")) >>
-    (fn idts => fold (fn idt => NuSys.assign_reg idt #> NuProcessor.process_no_input (Int.min (auto_level,1)) ctx) idts th))
+    (fn idts => fold (fn idt => NuSys.assign_reg ctx idt #> NuProcessor.process_no_input (Int.min (auto_level,1)) ctx) idts th))
 end\<close>
-\<nu>processor load_register 100 \<open>\<^bold>c\<^bold>u\<^bold>r\<^bold>r\<^bold>e\<^bold>n\<^bold>t blk \<^bold>r\<^bold>e\<^bold>s\<^bold>u\<^bold>l\<^bold>t\<^bold>s \<^bold>i\<^bold>n T\<close>  \<open>let open Parse in
-  safe (fn ctx => fn th => short_ident >> (fn idt => NuSys.load_reg idt th
+\<nu>processor  load_register 100 \<open>\<^bold>c\<^bold>u\<^bold>r\<^bold>r\<^bold>e\<^bold>n\<^bold>t blk \<^bold>r\<^bold>e\<^bold>s\<^bold>u\<^bold>l\<^bold>t\<^bold>s \<^bold>i\<^bold>n T\<close>  \<open>let open Parse in
+  safe (fn ctx => fn th => short_ident >> (fn idt => NuSys.load_reg ctx idt th
       handle NuRegisters.NoSuchRegister _ => raise Bypass))
 end\<close>
 \<nu>processor \<nu>simplifier 40 \<open>\<^bold>c\<^bold>u\<^bold>r\<^bold>r\<^bold>e\<^bold>n\<^bold>t blk \<^bold>r\<^bold>e\<^bold>s\<^bold>u\<^bold>l\<^bold>t\<^bold>s \<^bold>i\<^bold>n T\<close>  \<open>NuProcessors.simplifier\<close>
-\<nu>processor \<nu>autoprover 9000 \<open>P \<Longrightarrow> PROP Q\<close>  \<open>premise_prover (not_safe  Simpdata.auto_tac)\<close>
+\<nu>processor \<nu>autoprover 9000 \<open>P \<Longrightarrow> PROP Q\<close>
+  \<open>let open Tactical Method in 
+    premise_prover (not_safe (fn ctx => SOLVED' (K (ALLGOALS (insert_tac ctx (Proof_Context.get_thms ctx "that")) THEN Simpdata.auto_tac ctx)) 0))
+  end\<close>
+\<nu>processor call 9000 \<open>\<^bold>c\<^bold>u\<^bold>r\<^bold>r\<^bold>e\<^bold>n\<^bold>t blk \<^bold>r\<^bold>e\<^bold>s\<^bold>u\<^bold>l\<^bold>t\<^bold>s \<^bold>i\<^bold>n T\<close> \<open>safe (fn ctx => fn focus =>
+  Parse.position (Parse.short_ident || Parse.keyword || Parse.sym_ident) >> (fn proc =>
+    NuSys.apply_procs ctx (NuProcedure.check (Context.Proof ctx) proc) focus))\<close>
+
 \<nu>processor_resolver resolve_disposable 100  \<open>\<nu>Disposable T \<Longrightarrow> PROP P\<close> \<nu>disposable
 \<nu>processor_resolver resolve_share 100  \<open>Nu_Share N sh f \<Longrightarrow> PROP P\<close> \<nu>share
 end
