NuTest.thy
@@ -1,0 +1,587 @@
+theory NuTest
+  imports NuSys
+begin
+
+ML \<open>Name_Space.full_name (Name_Space.naming_of (Context.Proof @{context})) @{binding aaa}\<close>
+ML \<open>NuProcessor.defined (Context.Proof @{context}) "resolve_share"\<close>
+ML \<open>NuProcessor.get_attr (Context.Proof @{context}) ("resolve_share11", Position.none) 0\<close>
+ML \<open>curry (op ::)\<close>
+
+proc xxx: "(x \<tycolon> \<nat>[32] named x, y \<tycolon> \<nat>[32])" \<longmapsto> "(x + x + y \<tycolon> \<nat>[32])" for x :: nat  if A:"x < 100" and B:"y < 100" \<medium_left_bracket>
+  \<bullet> \<rightarrow> (x,y) x y +
+(* , x !!!  -- by (myrule \<nu>disposable) *)
+  thm \<nu>aux'raw
+
+
+(* 
+
+  \<nu>have xL10: "x < 10" 
+  have
+!!!  -- by (myrule \<nu>disposable)
+print_rules
+ML_val \<open>Context_Rules.print_rules @{context}\<close>
+term ?thesis
+  include show_more1 *)
+  
+(*  \<bullet> x y + !! -- by auto  \<bullet> 
+  \<bullet>  *)
+
+
+
+
+
+
+ML \<open>(fold o fold) Variable.declare_term\<close>
+ML \<open>(map o Proof_Context.cert_prop)\<close>
+ML \<open>
+local open Proof_Context in
+val prep_props = (map o cert_prop)
+val raw_args = [[]]
+val ctxt = @{context}
+    val props = prep_props ctxt (maps (map fst) raw_args);
+
+val patss = maps (map (prep_props (set_mode mode_pattern @{context}) o snd)) raw_args
+    val propps = unflat raw_args (props ~~ patss);
+
+end
+\<close>
+ML \<open>
+structure Data = Generic_Data
+(
+  type T = int Name_Space.table; (* key : the constant name, value: the definition *)
+  val empty: T = Name_Space.empty_table "\<nu>hehe";
+  val extend = I;
+  fun merge data : T = Name_Space.merge_tables data;
+);
+
+val _ =
+  Outer_Syntax.command \<^command_keyword>\<open>test\<close> "define \<nu>processor"
+      (Parse.name_position >> (fn x => Toplevel.proof (Proof.map_context  (fn ctx =>
+          let
+            val gtx = (Context.Proof ctx)
+            val tab =Data.get gtx
+val (x',a) = Name_Space.check gtx tab x 
+val _ = @{print} x'
+val _ = @{print} a
+in ctx end
+    ))));
+val _ =
+  Outer_Syntax.command \<^command_keyword>\<open>test2\<close> "define \<nu>processor"
+      (Scan.succeed () >> (fn _ => Toplevel.proof (Proof.map_contexts  (fn ctx =>
+let val data = Data.get (Context.Proof ctx)
+        val (_,tab2) = Name_Space.define (Context.Proof ctx) false (@{binding h1}, 233) data 
+in Context.proof_map (Data.put tab2) ctx end
+))))
+\<close>
+
+  notepad
+begin
+  fix P Q A :: bool
+  assume A: "A" and B: "Q" apply
+ML_val \<open>
+val th = Goal.init @{cprop "P"}
+val th2 = (ALLGOALS (Method.insert_tac @{context} @{thms A B}) THEN (auto_tac @{context} |> CHANGED_PROP)) th |> Seq.list_of
+\<close>
+end
+
+notepad
+begin
+
+  {
+    fix P :: bool
+    ML_prf \<open>Theory.local_setup (Proof_Context.bind_term (("x",0), @{term P}))\<close>
+    ML_prf \<open>Theory.local_setup (Proof_Context.put_thms false ("haha", SOME @{thms conjI}))\<close>
+
+test2
+    test h1
+    thm haha
+    term ?x
+    ML_prf \<open>Proof_Context.cert_term @{context} @{term "?x"}\<close>
+  
+
+    presume "P"
+    then have "P" .
+    note this
+  }
+test h1
+  ML_val \<open>burrow\<close>
+end
+  
+(*  \<nu> x y + ! by some \<nu> ! by some 
+  ML_val \<open>Thm.prop_of  @{thm this} \<close>
+  note conjI[\<nu>\<rho>_accept_proc]*)
+\<medium_right_bracket>
+
+ML \<open>val auto_method =
+  Scan.lift (Scan.option (Parse.nat -- Parse.nat)) --|
+    Method.sections clasimp_modifiers >>
+  (fn NONE => (fn ctx => SOLVED' (K (auto_tac ctx)) |> SIMPLE_METHOD')
+    | SOME (m, n) => (fn ctxt => SIMPLE_METHOD (CHANGED_PROP (mk_auto_tac ctxt m n))));
+val _ = Theory.setup (Method.setup \<^binding>\<open>myauto\<close> auto_method "myauto" #>
+Method.setup \<^binding>\<open>myrule\<close>
+      (Attrib.thms >> (fn rules => fn ctxt => METHOD (HEADGOAL o Method.some_rule_tac ctxt rules)))
+      "apply some intro/elim rule (potentially classical)")
+\<close>
+  notepad
+begin
+  fix A B C :: bool
+  assume A: A and B : "A \<Longrightarrow> C" and th2 : "D"
+  have "C  \<and> C" using B B apply (myrule conjI)
+    thm conjI[OF B]
+    (* using A B th2 apply myauto *)
+end
+
+
+
+
+term NuPrim.CodeBlock
+ML \<open>\<^const_name>\<open>CodeBlock\<close>\<close>
+term "NuPrim.CurrentConstruction"
+ML_val \<open>HOLogic.strip_tuple @{term "(A,B,C)"}\<close>
+proc "(x \<tycolon> \<nat>[32] named x, y \<tycolon> \<nat>[32])" for x :: nat \<medium_left_bracket> 
+    x y y + + 
+\<medium_right_bracket>
+ML_val \<open>NuBasics.mk_PropBlock 0 @{thm this}\<close>
+ML_val \<open>fold\<close>
+thm protectI
+thm PropBlock_I
+  \<rightarrow> x \<rightarrow> a \<rightarrow> p
+  note
+term y
+  fix xxx
+  term "xxx::nat"
+  term "xxx::bool"
+  ML_val \<open>@{term "a \<in> B"}\<close>
+term "\<R>"
+typ '\<R>
+\<medium_right_bracket>
+
+  
+
+ML_val \<open>
+val ctx = Proof_Context.set_mode Proof_Context.mode_schematic @{context}
+val (Term.Var xxx) = Syntax.read_term ctx "(?a::nat)"
+val tm1 = Syntax.read_term ctx "(A \<longrightarrow> X x \<longrightarrow> X x)"
+val tm2 = Syntax.read_term ctx "\<lambda>x z. (x  \<longrightarrow> z \<longrightarrow> z)"
+val x = Pattern.unify (Context.Proof ctx) (tm1,tm2) Envir.init
+val y = Envir.lookup x xxx
+\<close>
+
+
+
+ML \<open> 
+
+fun ctx_parser_wrap f (ctx,tok) = case f tok of (x,tok') => (x,(ctx,tok'))
+val ctx_parser_wrap : 'a parser -> 'a context_parser = ctx_parser_wrap
+fun thm_name ctx : Thm.binding parser
+   = Parse.binding -- (Parse.opt_attribs #>> map (Attrib.attribute_cmd ctx))
+val for_fixes : NuSyntax.fixes parser = Parse.for_fixes
+
+fun short_statement x =
+(  Parse_Spec.statement -- Parse_Spec.if_statement -- Parse.for_fixes
+    >> (fn ((shows, assumes), fixes) =>
+      (false, Binding.empty_atts, [], [Element.Fixes fixes, Element.Assumes assumes],
+        Element.Shows shows))) x;
+
+local open Parse in
+val arg_list = list (binding --| $$$ ":" -- (term -- term))
+val arg_list_p = $$$ "(" |-- arg_list --| $$$ ")"
+fun iden_with pred = Scan.one (pred o Token.content_of) >> Token.content_of;
+fun sym_iden_key x =
+  group (fn () => Token.str_of_kind Token.Sym_Ident ^ " " ^ quote x)
+    (iden_with (fn y => x = y));
+end
+
+
+val build = Parse.$$$ "\<medium_left_bracket>";
+val _ =
+  Outer_Syntax.local_theory_to_proof \<^command_keyword>\<open>proc\<close> "begin a procedure construction"
+    ((Parse.position Parse.term -- Parse.for_fixes -- Scan.optional Parse_Spec.includes []) --| build >> NuSys.begin_proc_cmd);
+val _ =
+  Outer_Syntax.command \<^command_keyword>\<open>block\<close> "begin a procedure construction"
+    ( build >> K (Toplevel.proof Proof.begin_block));
+val _ =
+  Outer_Syntax.command \<^command_keyword>\<open>\<lbrace>\<close> "begin a procedure construction"
+    ( build >> K (Toplevel.proof Proof.begin_block));
+
+val _ =
+  Outer_Syntax.command \<^command_keyword>\<open>finish\<close> "end context"
+    (Scan.succeed (Toplevel.proof Proof.end_block));
+
+val _ =
+  Outer_Syntax.command \<^command_keyword>\<open>\<medium_right_bracket>\<close> "end context"
+    (Scan.succeed
+      (Toplevel.exit o Toplevel.end_main_target o Toplevel.end_nested_target o
+        Toplevel.end_proof (K Proof.end_notepad #> (fn x => ( x)))));
+
+ \<close>
+
+notepad begin
+end
+
+term \<open>x \<tycolon> \<nat>[32] \<close>     
+
+
+
+
+
+
+
+(*   require "x < 100" and "y < 100"
+  x y + 10 + \<rightarrow> z
+  z' z *
+  cast 2 () *)
+
+value 1
+
+final_procedure pproc[] : "p \<nuLinkL>... \<nuLinkR> ..."
+
+lemma "P" proof -
+end
+
+
+
+ML_val \<open>
+  val s1 = "1"
+  val s2 = "2"
+  val t = Syntax.parse_term @{context} ("("^s1^","^s2^")")\<close>
+
+ML \<open>
+local
+
+val _ = Outer_Syntax.command \<^command_keyword>\<open>print_goal\<close> "print"
+    (Scan.succeed (Toplevel.proof (fn s =>
+      (@{print} (Proof.raw_goal s); s))));
+
+val _ =
+  Outer_Syntax.command \<^command_keyword>\<open>xnote\<close> "define facts"
+    (Parse_Spec.name_facts >> @{print} >> (Toplevel.proof o Proof.note_thmss_cmd));
+val long_keyword =
+  Parse_Spec.includes >> K "" ||
+  Parse_Spec.long_statement_keyword;
+
+val long_statement =
+  Scan.optional (Parse_Spec.opt_thm_name ":" --| Scan.ahead long_keyword) Binding.empty_atts --
+  Scan.optional Parse_Spec.includes [] -- Parse_Spec.long_statement
+    >> (fn ((binding, includes), (elems, concl)) => (true, binding, includes, elems, concl));
+
+val short_statement =
+  Parse_Spec.statement -- Parse_Spec.if_statement -- Parse.for_fixes
+    >> (fn ((shows, assumes), fixes) =>
+      (false, Binding.empty_atts, [], [Element.Fixes fixes, Element.Assumes assumes],
+        Element.Shows shows));
+
+fun theorem spec schematic descr =
+  Outer_Syntax.local_theory_to_proof' spec ("state " ^ descr)
+    ((long_statement || short_statement) >> (fn (long, binding, includes, elems, concl) =>
+      (@{print} (long, binding, includes, elems, concl);
+(if schematic then Specification.schematic_theorem_cmd else Specification.theorem_cmd)
+        long Thm.theoremK NONE (K I) binding includes elems concl)));
+val _ = theorem \<^command_keyword>\<open>xtheorem\<close> false "theorem";
+val _ = theorem \<^command_keyword>\<open>xlemma\<close> false "lemma";
+
+fun xdbg_proof prf = prf |> Proof.set_facts [@{thm conjI}]
+
+val _ =
+  Outer_Syntax.command \<^command_keyword>\<open>xdbg\<close> "begin explicit proof block"
+    (Scan.succeed (Toplevel.proof xdbg_proof));
+
+val structured_statement =
+  Parse_Spec.statement -- Parse_Spec.cond_statement -- Parse.for_fixes
+    >> (fn ((shows, (strict, assumes)), fixes) => (strict, fixes, assumes, shows));
+
+(* val _ =
+  Outer_Syntax.command \<^command_keyword>\<open>have\<close> "state local goal"
+    (structured_statement >> (fn (a, b, c, d) =>
+      Toplevel.proof' (fn int => Proof.have_cmd a NONE (K I) b c d int #> #2))); *)
+
+in end\<close>
+
+ML_val \<open> fold (fold (Proof_Context.augment o fst) o snd) \<close>
+
+xlemma "A + B = B" if "A = B" for A B :: nat 
+begin
+end_proc
+
+xlemma nth_equal_first_eq:
+  fixes x :: nat
+  notes conjI3 = conjI
+  assumes "x \<notin> set xs"
+  assumes "n \<le> length xs"
+  shows xx[]:"(x # xs) ! n = x \<longleftrightarrow> n = 0" (is "?lhs \<longleftrightarrow> ?rhs")
+proof
+  thm conjI3
+  print_goal
+  term ?lhs
+  assume ?lhs
+  show ?rhs
+  proof (rule ccontr)
+    assume "n \<noteq> 0"
+    then have "n > 0" by simp
+    with \<open>?lhs\<close> have "xs ! (n - 1) = x" by simp
+    moreover from \<open>n > 0\<close> \<open>n \<le> length xs\<close> have "n - 1 < length xs" by simp
+    ultimately have "\<exists>i<length xs. xs ! i = x" by auto
+    with \<open>x \<notin> set xs\<close> in_set_conv_nth [of x xs] show False by simp
+  qed
+next
+  assume ?rhs then show ?lhs by simp
+qed
+
+
+ML \<open>local open Parse in
+val is_props = Scan.repeat1 ($$$ "is" |-- prop);
+ val propp = Parse.prop -- Scan.optional ($$$ "(" |-- !!! (is_props --| $$$ ")")) []
+end\<close>
+ML \<open> Parse.and_list1  \<close>
+
+interface pproc[simp] : "sss"
+
+
+ML \<open> 
+
+local
+
+val thm_name = Parse_Spec.thm_name ":" #>> apsnd (map (Attrib.attribute_cmd ctx))
+
+val _ =
+  Outer_Syntax.local_theory_to_proof \<^command_keyword>\<open>mkproc\<close> "begin a procedure construction"
+    ((Parse_Spec.thm_name "+" >> \<^print>) |-- Parse.begin >> K Proof.begin_notepad);
+
+in end \<close>
+
+  note
+
+ML_val \<open>
+op ||>
+ \<close>
+
+  ML_val \<open>
+Parse.and_list1;
+ (--) \<close>
+
+ML_val \<open>
+local open Proof in
+fun these_factss more_facts (named_factss, state) =
+  (named_factss, state |> set_facts (maps snd named_factss @ more_facts));
+
+fun gen_thmss more_facts opt_chain opt_result prep_atts prep_fact args state =
+  state
+  |> assert_forward
+  |> map_context_result (fn ctxt => ctxt |> Proof_Context.note_thmss ""
+    (Attrib.map_facts_refs (map (prep_atts ctxt)) (prep_fact ctxt) args))
+  |> these_factss (more_facts state)
+  ||> opt_chain
+  |> opt_result;
+end
+
+val local_results = gen_thmss (K []) I I (K I) (K I) o map (apsnd Thm.simple_fact);x`
+  \<close>
+
+ML_val \<open>
+fun empty_bindings args = map (pair Binding.empty_atts) args; \<close>
+
+lemma "P \<and> Q" if asm: "Q \<and> P" for P Q :: bool
+proof (rule conjI)
+  from that have a:"P" and b:"Q" by (blast, blast)
+  with this print_goal
+   have "Q" using b 
+    print_goal
+    by fast
+  print_goal
+  thm this
+  xdbg
+  thm this
+  print_goal
+end
+
+notepad begin
+  print_goal
+end
+
+
+  {
+ML_val \<open> (true ? (fn x => x +  1)) 1 \<close>
+lemma x:"x = x" proof qed
+
+  
+  ML_val \<open>
+    val th1 = Thm.assume @{cterm "\<And>x y. P x y"}
+    val th3 = Drule.forall_elim_list [Thm.cterm_of @{context} (Var (("aa",1),@{typ 'a}))] th1
+    val th2 = Drule.infer_instantiate @{context} [(("?x",0), @{cterm "x::'a"})] th1
+(* (Drule.forall_intr_vars  @{thm as}) *)
+ \<close>
+
+
+lemma
+  assumes asm: "P"
+  shows th: "P"
+proof -
+  from asm show ?thesis by this
+qed
+
+thm th
+value "len_of (TYPE (2))"
+
+lemma ex: "A \<and> B \<longrightarrow> B \<and> A"
+proof
+  assume "A \<and> B"
+  then obtain B and A ..
+  then show "B \<and> A" ..
+qed
+
+notepad begin
+  include show_more
+  fix P Q A B C :: bool
+  assume t1: "P \<Longrightarrow> A \<Longrightarrow> P \<Longrightarrow> Q"
+  ML_val \<open> Simplifier.norm_hhf @{context} @{thm t1} \<close>
+  assume t2: "B \<Longrightarrow> C \<Longrightarrow> P"
+  assume t3: "A \<Longrightarrow> (P \<Longrightarrow> Q \<Longrightarrow> C)"
+  assume t4: "A"
+  note t1[OF t2]
+  note x1 = t1[OF t2 t4]
+
+  thm conjI
+  ML_val \<open>
+  val thm = @{thm x1};
+val prf = Thm.proof_of thm
+
+ \<close>
+
+
+
+  thm t1
+  have t1: "B \<Longrightarrow> C \<Longrightarrow> P" using t2 by this
+  thm t1
+
+  ML_val \<open>
+type lthy =
+ {background_naming: Name_Space.naming,
+  operations: Local_Theory.operations,
+  conclude: Proof.context -> Proof.context,
+  target: Proof.context};
+structure Data = Proof_Data
+(
+  type T = lthy list;
+  fun init _ = [];
+);
+val x = hd o Data.get
+val y = Binding.name
+
+\<close>
+
+  ML_val \<open>
+val zz= Facts.dest_all (Context.Proof @{context}) false []
+  (Proof_Context.facts_of @{context})
+\<close>
+
+  have "\<And> x. P x"
+proof -
+    have "P x" for x sorry
+  thus "\<And> x. P x"
+    by fast
+qed
+
+  assume as:"\<And>x y. P x y" 
+  thm as
+  ML_val \<open>
+   Thm.tpairs_of ( (Goal.init @{cterm "PROP PP"}))
+\<close>
+  {
+    fix x :: "'a"
+    {
+      have "x \<equiv> x" by (rule reflexive)
+    }
+    thm this
+  }
+  
+end
+
+context 
+  includes show_more
+  fixes P :: "'a \<Rightarrow> bool"
+  assumes as:"\<And>x. P x" 
+begin
+
+  
+
+ML_val \<open>
+val prep_att = Attrib.check_src
+val lthy = @{context}
+val ((name, raw_atts),raw_includes,raw_elems,raw_concl,int) = 
+val y = (Element.map_ctxt_attrib (prep_att lthy)) 
+val x = Local_Theory.assert  @{context}\<close>
+  xlemma x: "P \<and> Q" and y:"P" if "Q" for Q :: bool by (simp add: as add: that)+
+end
+
+
+notepad begin
+  fix P Q A B C :: bool
+  fix S T :: "'a \<Rightarrow> bool"
+  assume x: "P = Q"
+  assume A: "P \<Longrightarrow> P \<Longrightarrow> Q"
+  assume B: "A \<Longrightarrow> B \<Longrightarrow> C"
+  assume C: "P \<Longrightarrow> P \<longrightarrow> Q"
+  assume D: "\<forall>x. S x \<longrightarrow> T x"
+  include show_more
+  thm ac_simps
+  have ac_simps: "P = Q" by (simp add: x)
+thm ac_simps
+  thm spec
+  note d = mp[OF spec[OF D]]
+  ML_val \<open>
+local
+val ctxt = @{context}
+val facts = Proof_Context.facts_of @{context}
+val x = Global_Theory.facts_of (Proof_Context.theory_of ctxt)
+in
+val f2 = Facts.dest_static true [x] facts;
+val f1= (Facts.props facts)
+   end
+  
+\<close>
+
+  ML_val \<open>
+structure Data = Generic_Data
+(
+  type T = thm Item_Net.T;
+  val empty = Thm.full_rules;
+  val extend = I;
+  val merge = Item_Net.merge;
+);
+val content = Item_Net.content o Data.get;\<close>
+  ML_val \<open> Symtab.lookup \<close>
+
+  ML_val \<open> 
+  val th3 = Thm.RS (@{thm spec}, @{thm D})
+(*  val th2 = Thm.RS (@{thm spec}, @{thm D}) *)
+  val th1 = Thm.assume @{cterm "P \<Longrightarrow> W"}
+  val xx1 = Thm.RS ( @{thm mp}, @{thm B})
+ (* val tP = @{cterm "HOL.Trueprop P"}
+  val th1 = Thm.assume tP
+  val th2 = Drule.OF (@{thm A}, [th1,th1])
+  val th3 = Thm.implies_intr tP (Thm.implies_elim (Thm.implies_elim @{thm A} th1) th1) *) \<close>
+  
+ML_val \<open> Thm.get_tags (Thm.put_name_hint "s" @{thm x})\<close>
+ML_val \<open>
+local val fc = Proof_Context.facts_of @{context}
+  val names = map #1 (Facts.dest_all (Context.Proof @{context}) false [] fc)
+in
+  val x = map @{print} (filter (Facts.is_dynamic fc) names)
+end \<close>
+  note x[symmetric]
+  xnote y[simp] = x[symmetric] \<open>P = Q\<close>
+    and z = x
+  note ac_simps = y
+  
+  
+end
+
+mkproc asd[simp]+ begin
+
+ML_val \<open> @{Isar.state} \<close>
+  ML_val \<open> Proof.init ( \<^context>) \<close>
+
+  have
+  note this
+end
+end
